examples/ghc/lib/CoreArity.v
@@ -17,7 +17,6 @@ Require BasicTypes.
 Require Core.
 Require CoreUtils.
 Require GHC.Base.
-Require GHC.Core.TyCo.Subst.
 Require GHC.Types.Cpr.
 Require HsToCoq.Err.
 Require UnVarGraph.
@@ -262,9 +261,7 @@ Axiom etaBodyForJoinPoint : nat ->
                             Core.CoreExpr -> (list Core.CoreBndr * Core.CoreExpr)%type.
 
 Axiom freshEtaId : nat ->
-                   GHC.Core.TyCo.Subst.Subst ->
-                   Core.Scaled AxiomatizedTypes.Type_ ->
-                   (GHC.Core.TyCo.Subst.Subst * Core.Id)%type.
+                   Core.Subst -> Core.Scaled AxiomatizedTypes.Type_ -> (Core.Subst * Core.Id)%type.
 
 (* External variables:
      bool list nat op_zt__ option AxiomatizedTypes.Coercion AxiomatizedTypes.Type_
@@ -272,8 +269,8 @@ Axiom freshEtaId : nat ->
      BasicTypes.OneShotInfo BasicTypes.RecFlag Core.Card Core.CoercionR Core.CoreArg
      Core.CoreBndr Core.CoreExpr Core.CoreRule Core.DataCon Core.Divergence
      Core.DmdSig Core.ForAllTyBinder Core.Id Core.IdEnv Core.InScopeSet
-     Core.MCoercion Core.MCoercionR Core.Scaled Core.SubDemand Core.Var
-     CoreUtils.CheapAppFun GHC.Base.String GHC.Core.TyCo.Subst.Subst
-     GHC.Types.Cpr.CprSig HsToCoq.Err.Build_Default HsToCoq.Err.Default
-     HsToCoq.Err.default UnVarGraph.UnVarSet Util.HasDebugCallStack
+     Core.MCoercion Core.MCoercionR Core.Scaled Core.SubDemand Core.Subst Core.Var
+     CoreUtils.CheapAppFun GHC.Base.String GHC.Types.Cpr.CprSig
+     HsToCoq.Err.Build_Default HsToCoq.Err.Default HsToCoq.Err.default
+     UnVarGraph.UnVarSet Util.HasDebugCallStack
 *)
