examples/ghc/module-edits/CSE/midamble.v
@@ -1,4 +1,4 @@
 Require NestedRecursionHelpers.
 
 (* default = emptyCSEnv *)
-#[global] Instance Default__CSEnv : HsToCoq.Err.Default CSEnv := {| HsToCoq.Err.default := CS GHC.Core.TyCo.Subst.emptySubst GHC.Core.Map.Expr.emptyCoreMap GHC.Core.Map.Expr.emptyCoreMap |}.
+#[global] Instance Default__CSEnv : HsToCoq.Err.Default CSEnv := {| HsToCoq.Err.default := CS Core.emptySubst GHC.Core.Map.Expr.emptyCoreMap GHC.Core.Map.Expr.emptyCoreMap |}.
